examples/CCS/ExampleScript.sml
@@ -29,112 +29,13 @@ val _ = disable_tyabbrev_printing "simulation";
 
 (******************************************************************************)
 (*                                                                            *)
-(*          The proof of PROPERTY_STAR (old way as in Milner's book)          *)
+(*                     The coffee machine model [2]                           *)
 (*                                                                            *)
 (******************************************************************************)
 
-(*
- In StrongEQScript.ml, currently we define STRONG_EQUIV (strong bisimilarity) by
- HOL's co-inductive package (Hol_coreln):
-
-val (STRONG_EQUIV_rules, STRONG_EQUIV_coind, STRONG_EQUIV_cases) = Hol_coreln `
-    (!(E :('a, 'b) CCS) (E' :('a, 'b) CCS).
-       (!u.
-         (!E1. TRANS E u E1 ==>
-               (?E2. TRANS E' u E2 /\ STRONG_EQUIV E1 E2)) /\
-         (!E2. TRANS E' u E2 ==>
-               (?E1. TRANS E u E1 /\ STRONG_EQUIV E1 E2))) ==> STRONG_EQUIV E E')`;
-
-  then the 3rd returned value (STRONG_EQUIV_cases) is just the PROPERTY_STAR:
-
-(* Prop. 4, page 91: strong equivalence satisfies property [*] *)
-val PROPERTY_STAR = save_thm ((* NEW *)
-   "PROPERTY_STAR", STRONG_EQUIV_cases);
-
- However, if we started with the original definition of STRONG_EQUIV, which now
- becomes a theorem:
-
-val STRONG_EQUIV = new_definition (
-   "STRONG_EQUIV",
-  ``STRONG_EQUIV E E' = ?Bsm. Bsm E E' /\ STRONG_BISIM Bsm``);
-
- It's not easy to prove PROPERTY_STAR, below is the proof of Robin Milner through
- a temporarily definition STRONG_EQUIV', originally formalized by Monica Nesi.
-
- *)
-
-(* Definition 3, page 91 in Milner's book. *)
-val STRONG_EQUIV' = new_definition (
-   "STRONG_EQUIV'",
-  ``STRONG_EQUIV' E E' =
-        (!u.
-         (!E1. TRANS E u E1 ==>
-               (?E2. TRANS E' u E2 /\ STRONG_EQUIV E1 E2)) /\
-         (!E2. TRANS E' u E2 ==>
-               (?E1. TRANS E u E1 /\ STRONG_EQUIV E1 E2)))``);
-
-(* Strong equivalence implies the new relation. *)
-val STRONG_EQUIV_IMP_STRONG_EQUIV' = store_thm (
-   "STRONG_EQUIV_IMP_STRONG_EQUIV'",
-      ``!E E'. STRONG_EQUIV E E' ==> STRONG_EQUIV' E E'``,
-    rpt GEN_TAC
- >> REWRITE_TAC [STRONG_EQUIV', STRONG_EQUIV]
- >> rpt STRIP_TAC (* 2 sub-goals *)
- >> IMP_RES_TAC
-      (MATCH_MP (EQ_MP STRONG_BISIM (ASSUME ``STRONG_BISIM Bsm``))
-                (ASSUME ``(Bsm: ('a, 'b) simulation) E E'``))
- >| [ Q.EXISTS_TAC `E2`,
-      Q.EXISTS_TAC `E1` ]
- >> ASM_REWRITE_TAC []
- >> Q.EXISTS_TAC `Bsm`
- >> ASM_REWRITE_TAC [] );
-
-val STRONG_EQUIV'_IS_STRONG_BISIM = store_thm (
-   "STRONG_EQUIV'_IS_STRONG_BISIM",
-  ``STRONG_BISIM STRONG_EQUIV'``,
-    PURE_ONCE_REWRITE_TAC [STRONG_BISIM]
- >> rpt STRIP_TAC (* 2 sub-goals here *)
- >> IMP_RES_TAC
-       (EQ_MP (Q.SPECL [`E`, `E'`] STRONG_EQUIV')
-              (ASSUME ``STRONG_EQUIV' E E'``))
- >| [ Q.EXISTS_TAC `E2`,
-      Q.EXISTS_TAC `E1` ]
- >> IMP_RES_TAC STRONG_EQUIV_IMP_STRONG_EQUIV'
- >> ASM_REWRITE_TAC []);
-
-(* The new relation implies strong equivalence. *)
-val STRONG_EQUIV'_IMP_STRONG_EQUIV = store_thm (
-   "STRONG_EQUIV'_IMP_STRONG_EQUIV",
-      ``!E E'. STRONG_EQUIV' E E' ==> STRONG_EQUIV E E'``,
-    rpt STRIP_TAC
- >> PURE_ONCE_REWRITE_TAC [STRONG_EQUIV]
- >> EXISTS_TAC ``STRONG_EQUIV'``
- >> ASM_REWRITE_TAC [STRONG_EQUIV'_IS_STRONG_BISIM]);
-
-(* Prop. 4, page 91: strong equivalence satisfies property [*] *)
-val PROPERTY_STAR' = store_thm (
-   "PROPERTY_STAR'",
-      ``!E E'. STRONG_EQUIV E E' =
-         (!u.
-           (!E1. TRANS E u E1 ==>
-                 (?E2. TRANS E' u E2 /\ STRONG_EQUIV E1 E2)) /\
-           (!E2. TRANS E' u E2 ==>
-                 (?E1. TRANS E u E1 /\ STRONG_EQUIV E1 E2)))``,
-    rpt GEN_TAC
- >> EQ_TAC (* 2 sub-goals here *)
- >| [ PURE_ONCE_REWRITE_TAC
-        [ONCE_REWRITE_RULE [STRONG_EQUIV'] STRONG_EQUIV_IMP_STRONG_EQUIV'],
-      PURE_ONCE_REWRITE_TAC
-        [ONCE_REWRITE_RULE [STRONG_EQUIV'] STRONG_EQUIV'_IMP_STRONG_EQUIV] ]);
-
-(******************************************************************************)
-(*                                                                            *)
-(*                     The coffee machine model                               *)
-(*                                                                            *)
-(******************************************************************************)
-
-val VM = ``rec "VM" (In "coin"..(In "ask-esp"..rec "VM1" (Out "esp-coffee"..var "VM") +
-                                 In "ask-am"..rec "VM2" (Out "am-coffee"..var "VM")))``;
+val VM = “rec "VM" (In "coin"..
+                      (In "ask-esp"..rec "VM1" (Out "esp-coffee"..var "VM") +
+                       In "ask-am"..rec "VM2" (Out "am-coffee"..var "VM")))”;
 
 (* ex1 =
 |- label (name "a")..label (name "b")..nil +
@@ -196,7 +97,8 @@ val List_eq_coList = store_thm (
 (******************************************************************************)
 
 local
-    val (temp_A, trans) = CCS_TRANS ``label (name "a")..nil || label (coname "a")..nil``;
+    val (temp_A, trans) =
+        CCS_TRANS “label (name "a")..nil || label (coname "a")..nil”;
     val nodes = map (fn (l, s) => CCS_TRANS s) trans;
 in
   val ex_A = save_thm ("ex_A", temp_A);
@@ -269,4 +171,9 @@ val _ =
  else
     {};
 
-(* last updated: Oct 15, 2017 *)
+(* Bibliography:
+
+ [1] Milner, Robin. Communication and concurrency. Prentice hall, 1989.
+ [2] Gorrieri, R., Versari, C.: Introduction to Concurrency Theory. Springer (2015).
+
+ *)
