examples/lambda/basics/ctermScript.sml
@@ -1,6 +1,6 @@
 open HolKernel Parse boolLib bossLib;
 
-open boolSimps arithmeticTheory pred_setTheory finite_mapTheory hurdUtils;
+open boolSimps arithmeticTheory pred_setTheory listTheory finite_mapTheory hurdUtils;
 
 open generic_termsTheory binderLib nomsetTheory nomdatatype;
 
@@ -8,7 +8,9 @@ val _ = new_theory "cterm";
 
 val tyname = "cterm"
 
-val vp = ``(λn u:unit. n = 0)``
+val vp = “(λn u:unit. n = 0)”;
+
+(* GLAM corresponds to APP, LAM and CONST *)
 val lp = “(λn (d:unit + unit + 'a) tns uns.
              n = 0 ∧ ISL d ∧ tns = [] ∧ uns = [0;0] ∨
              n = 0 ∧ ISR d ∧ ISL (OUTR d) ∧ tns = [0] ∧ uns = [] ∨
@@ -27,7 +29,6 @@ val LAM_termP = prove(
   mk_comb(termP, LAM_def |> SPEC_ALL |> concl |> rhs |> rand),
   match_mp_tac glam >> srw_tac [][genind_term_REP]);
 val LAM_t = defined_const LAM_def
-
 
 val APP_t = mk_var("APP", ``:^newty -> ^newty -> ^newty``)
 val APP_def = new_definition(
@@ -191,16 +192,6 @@ val tlf =
                 (cterm_ABS (HD (TL ts2))) p: 'r``
 val tvf = ``λ(s:string) (u:unit) (p:ρ). tvf s p : 'r``
 
-val LENGTH_NIL' =
-    CONV_RULE (BINDER_CONV (LAND_CONV (REWR_CONV EQ_SYM_EQ)))
-              listTheory.LENGTH_NIL
-val LENGTH1 = prove(
-  ``(1 = LENGTH l) ⇔ ∃e. l = [e]``,
-  Cases_on `l` >> srw_tac [][listTheory.LENGTH_NIL]);
-val LENGTH2 = prove(
-  ``(2 = LENGTH l) ⇔ ∃a b. l = [a;b]``,
-  Cases_on `l` >> srw_tac [][LENGTH1]);
-
 val termP_elim = prove(
   ``(∀g. ^termP g ⇒ P g) ⇔ (∀t. P (^term_REP_t t))``,
   srw_tac [][EQ_IMP_THM] >- srw_tac [][genind_term_REP] >>
@@ -236,10 +227,9 @@ val parameter_tm_recursion = save_thm(
                                LIST_REL_CONS1, genind_GVAR,
                                genind_GLAM_eqn, sidecond_def,
                                NEWFCB_def, relsupp_def,
-                               LENGTH_NIL', LENGTH1, LENGTH2]
+                               LENGTH_NIL_SYM, LENGTH1, LENGTH2]
       |> ONCE_REWRITE_RULE [termP0]
-      |> SIMP_RULE (srw_ss() ++ DNF_ss) [LENGTH1, LENGTH2,
-                                         listTheory.LENGTH_NIL]
+      |> SIMP_RULE (srw_ss() ++ DNF_ss) [LENGTH1, LENGTH2, LENGTH_NIL]
       |> CONV_RULE (DEPTH_CONV termP_removal)
       |> SIMP_RULE (srw_ss()) [GSYM supp_tpm, SYM term_REP_tpm]
       |> UNDISCH
@@ -258,25 +248,6 @@ val parameter_tm_recursion = save_thm(
                  `dpm` |-> `apm`, ‘tcf’ |-> ‘cn’]
       |> CONV_RULE (REDEPTH_CONV sort_uvars))
 
-val FORALL_ONE = prove(
-  ``(!u:one. P u) = P ()``,
-  SRW_TAC [][EQ_IMP_THM, oneTheory.one_induction]);
-val FORALL_ONE_FN = prove(
-  ``(!uf : one -> 'a. P uf) = !a. P (\u. a)``,
-  SRW_TAC [][EQ_IMP_THM] THEN
-  POP_ASSUM (Q.SPEC_THEN `uf ()` MP_TAC) THEN
-  Q_TAC SUFF_TAC `(\y. uf()) = uf` THEN1 SRW_TAC [][] THEN
-  SRW_TAC [][FUN_EQ_THM, oneTheory.one]);
-
-val EXISTS_ONE_FN = prove(
-  ``(?f : 'a -> one -> 'b. P f) = (?f : 'a -> 'b. P (\x u. f x))``,
-  SRW_TAC [][EQ_IMP_THM] THENL [
-    Q.EXISTS_TAC `\a. f a ()` THEN SRW_TAC [][] THEN
-    Q_TAC SUFF_TAC `(\x u. f x ()) = f` THEN1 SRW_TAC [][] THEN
-    SRW_TAC [][FUN_EQ_THM, oneTheory.one],
-    Q.EXISTS_TAC `\a u. f a` THEN SRW_TAC [][]
-  ]);
-
 val ctm_recursion = save_thm(
   "ctm_recursion",
   parameter_tm_recursion
@@ -284,8 +255,8 @@ val ctm_recursion = save_thm(
       |> Q.INST [`ppm` |-> `discrete_pmact`, `vr` |-> `λs u. vru s`,
                  `ap` |-> `λr1 r2 t1 t2 u. apu (r1()) (r2()) t1 t2`,
                  `lm` |-> `λr v t u. lmu (r()) v t`]
-      |> SIMP_RULE (srw_ss()) [FORALL_ONE, FORALL_ONE_FN, EXISTS_ONE_FN,
-                               fnpm_def]
+      |> SIMP_RULE (srw_ss()) [oneTheory.FORALL_ONE, oneTheory.FORALL_ONE_FN,
+                               oneTheory.EXISTS_ONE_FN, fnpm_def]
       |> SIMP_RULE (srw_ss() ++ CONJ_ss) [supp_unitfn]
       |> Q.INST [`apu` |-> `ap`, `lmu` |-> `lm`, `vru` |-> `vr`])
 
@@ -1041,3 +1012,4 @@ val _ = adjoin_after_completion (fn _ => PP.add_string term_info_string)
 
 
 val _ = export_theory()
+val _ = html_theory "cterm";
